src/Specific/ArithmeticSynthesisFramework.v
@@ -1,0 +1,643 @@
+Require Import Coq.ZArith.ZArith Coq.ZArith.BinIntDef.
+Require Import Coq.Lists.List. Import ListNotations.
+Require Import Crypto.Arithmetic.Core. Import B.
+Require Import Crypto.Arithmetic.PrimeFieldTheorems.
+Require Import Crypto.Arithmetic.Saturated.Freeze.
+Require Crypto.Specific.CurveParameters.
+Require Import Crypto.Util.Decidable.
+Require Import Crypto.Util.LetIn Crypto.Util.ZUtil.
+Require Import Crypto.Util.Tactics.BreakMatch.
+Require Import Crypto.Util.Tactics.TransparentAssert.
+Require Crypto.Util.Tuple.
+Require Import Crypto.Util.QUtil.
+Require Import Crypto.Util.ZRange Crypto.Util.BoundedWord.
+Require Import Crypto.Util.FixedWordSizes.
+Require Import Crypto.Util.Tactics.DestructHead.
+Local Notation tuple := Tuple.tuple.
+Local Open Scope list_scope.
+Local Open Scope Z_scope.
+Local Coercion Z.of_nat : nat >-> Z.
+
+Section wt.
+  Import QArith Qround.
+  Local Coercion QArith_base.inject_Z : Z >-> Q.
+  Definition wt_gen (m : positive) (sz : nat) (i:nat) : Z := 2^Qceiling((Z.log2_up m/sz)*i).
+End wt.
+
+Module Export Package.
+  Local Infix "^" := tuple : type_scope.
+
+  Class ArithmeticSynthesisTestParams :=
+    {
+      m : positive;
+      sz : nat;
+      a24 : Z;
+      lgbitwidth : nat;
+      adjusted_bitwidth : nat;
+      bounds : Tuple.tuple zrange sz;
+      allowable_bit_widths : list nat;
+      freeze_allowable_bit_widths : list nat;
+    }.
+
+  Class ArithmeticSynthesisTestPackage' {TP : ArithmeticSynthesisTestParams} :=
+    {
+      wt : nat -> Z
+      := wt_gen m sz;
+
+      a24_sig
+      : { a24t : Z ^ sz
+        | Positional.Fdecode wt a24t = F.of_Z m a24 };
+      add_sig
+      : { add : Z ^ sz -> Z ^ sz -> Z ^ sz
+        | forall a b : Z ^ sz,
+            let eval := Positional.Fdecode (m:=m) wt in
+            eval (add a b) = (eval a + eval b)%F };
+      sub_sig
+      : { sub : Z ^ sz -> Z ^ sz -> Z ^ sz
+        | forall a b : Z ^ sz,
+            let eval := Positional.Fdecode (m:=m) wt in
+            eval (sub a b) = (eval a - eval b)%F };
+      opp_sig
+      : { opp : Z ^ sz -> Z ^ sz
+        | forall a : Z ^ sz,
+            let eval := Positional.Fdecode (m:=m) wt in
+            eval (opp a) = F.opp (eval a) };
+      mul_sig
+      : { mul : Z ^ sz -> Z ^ sz -> Z ^ sz
+        | forall a b : Z ^ sz,
+            let eval := Positional.Fdecode (m:=m) wt in
+            eval (mul a b) = (eval a * eval b)%F };
+      square_sig
+      : { square : Z ^ sz -> Z ^ sz
+        | forall a : Z ^ sz,
+            let eval := Positional.Fdecode (m:=m) wt in
+            eval (square a) = (eval a * eval a)%F };
+      carry_sig
+      : { carry : Z ^ sz -> Z ^ sz
+        | forall a : Z ^ sz,
+            let eval := Positional.Fdecode (m:=m) wt in
+            eval (carry a) = eval a };
+      freeze_sig
+      : { freeze : Z ^ sz -> Z ^ sz
+        | forall a : Z ^ sz,
+            (0 <= Positional.eval wt a < 2 * Z.pos m)->
+            let eval := Positional.Fdecode (m:=m) wt in
+            eval (freeze a) = eval a };
+
+      feW
+      := Tuple.tuple (wordT lgbitwidth) sz;
+      feBW
+      := BoundedWord sz adjusted_bitwidth bounds;
+
+      phiW : feW -> F m
+      := fun x => B.Positional.Fdecode wt (Tuple.map wordToZ x);
+      phiBW : feBW -> F m
+      := fun x => B.Positional.Fdecode wt (BoundedWordToZ _ _ _ x);
+
+      feW_bounded : feW -> Prop;
+
+      feBW_to_Z : feBW -> tuple Z sz;
+      feBW_bounded : forall (a : feBW),
+          0 <= B.Positional.eval wt (feBW_to_Z a) < 2 * Z.pos m;
+    }.
+
+  Class > ArithmeticSynthesisTestPackage
+    := { ASParams :> ArithmeticSynthesisTestParams;
+         ASPackage :> @ArithmeticSynthesisTestPackage' ASParams }.
+  Coercion ASPackage : ArithmeticSynthesisTestPackage >-> ArithmeticSynthesisTestPackage'.
+  Coercion ASParams : ArithmeticSynthesisTestPackage >-> ArithmeticSynthesisTestParams.
+  Coercion Build_ArithmeticSynthesisTestPackage : ArithmeticSynthesisTestPackage' >-> ArithmeticSynthesisTestPackage.
+
+  Declare Reduction package_red
+    := cbv [m
+              ASParams
+              ASPackage
+              sz
+              a24
+              wt
+              a24_sig
+              add_sig
+              sub_sig
+              opp_sig
+              mul_sig
+              square_sig
+              carry_sig
+              lgbitwidth
+              adjusted_bitwidth
+              bounds
+              feW
+              feBW
+              phiW
+              phiBW
+              feW_bounded
+              feBW_to_Z
+              feBW_bounded
+              allowable_bit_widths
+              freeze_allowable_bit_widths].
+End Package.
+
+Module Synthesize (Curve : CurveParameters.CurveParameters).
+  Hint Opaque freeze : uncps.
+  Hint Rewrite freeze_id : uncps.
+
+  Module Import Internal.
+    Module P := CurveParameters.FillCurveParameters Curve.
+
+    Local Infix "^" := tuple : type_scope.
+
+    (* These definitions will need to be passed as Ltac arguments (or
+     cleverly inferred) when things are eventually automated *)
+    Ltac pose_computed Pv v :=
+      let v' := P.do_compute Pv in
+      pose v' as v.
+    Ltac pose_unfolded Pv v :=
+      let v' := P.do_unfold Pv in
+      pose v' as v.
+    Ltac pose_sz sz := pose_computed P.sz sz.
+    Ltac pose_bitwidth bitwidth := pose_computed P.bitwidth bitwidth.
+    Ltac pose_s s := pose_unfolded P.s s. (* don't want to compute, e.g., [2^255] *)
+    Ltac pose_c c := pose_computed P.c c.
+    Ltac pose_carry_chain1 carry_chain1 := pose_computed P.carry_chain1 carry_chain1.
+    Ltac pose_carry_chain2 carry_chain2 := pose_computed P.carry_chain2 carry_chain2.
+
+    Ltac pose_a24 a24 := pose_computed P.a24 a24.
+
+    Ltac pose_coef_div_modulus coef_div_modulus :=
+      pose_computed P.coef_div_modulus coef_div_modulus.
+
+    (* These definitions are inferred from those above *)
+    Ltac pose_m s c m :=  (* modulus *)
+      let m' := (eval vm_compute in (Z.to_pos (s - Associational.eval c))) in
+      pose m' as m.
+
+    Ltac pose_wt m sz wt :=
+      let wt' := (eval cbv [wt_gen] in (wt_gen m sz)) in
+      pose wt' as wt.
+    Ltac pose_sz2 sz sz2 :=
+      let sz2' := (eval vm_compute in ((sz * 2) - 1)%nat) in
+      pose sz2' as sz2.
+    Ltac pose_m_enc sz wt s c m_enc :=
+      let m_enc' := (eval vm_compute in (Positional.encode (modulo:=modulo) (div:=div) (n:=sz) wt (s-Associational.eval c))) in
+      let m_enc' := (eval cbv in m_enc') in (* compute type arguments *)
+      pose m_enc' as m_enc.
+    Ltac pose_coef sz wt m_enc coef_div_modulus coef := (* subtraction coefficient *)
+      let coef' := (eval vm_compute in
+                       ((fix addm (acc: Z^sz) (ctr : nat) : Z^sz :=
+                           match ctr with
+                           | O => acc
+                           | S n => addm (Positional.add_cps wt acc m_enc id) n
+                           end) (Positional.zeros sz) coef_div_modulus)) in
+      let coef' := (eval cbv in coef') in (* compute type arguments *)
+      pose coef' as coef.
+    Ltac pose_coef_mod m sz wt coef coef_mod :=
+      pose (eq_refl : mod_eq m (Positional.eval (n:=sz) wt coef) 0) as coef_mod.
+    Ltac pose_sz_nonzero sz sz_nonzero :=
+      assert (sz_nonzero : sz <> 0%nat) by (clear; abstract vm_decide).
+    Ltac pose_wt_nonzero wt wt_nonzero :=
+      assert (wt_nonzero : forall i, wt i <> 0)
+      by (clear; abstract (eapply pow_ceil_mul_nat_nonzero; vm_decide)).
+    Ltac pose_wt_divides wt wt_divides :=
+      assert (wt_divides : forall i, wt (S i) / wt i > 0)
+      by (clear; abstract (apply pow_ceil_mul_nat_divide; vm_decide)).
+    Ltac pose_wt_divides' wt wt_divides wt_divides' :=
+      assert (wt_divides' : forall i, wt (S i) / wt i <> 0)
+      by (clear -wt_divides; abstract (symmetry; apply Z.lt_neq, Z.gt_lt_iff, wt_divides)).
+    Ltac pose_wt_divides_chain carry_chain wt wt_divides' wt_divides_chain :=
+      assert (wt_divides_chain : forall i (H:In i carry_chain), wt (S i) / wt i <> 0)
+      by (clear -wt_divides'; abstract (let i := fresh "i" in intros i ?; exact (wt_divides' i))).
+
+    Local Ltac solve_constant_sig sz wt :=
+      lazymatch goal with
+      | [ |- { c : Z^?sz | Positional.Fdecode (m:=?M) ?wt c = ?v } ]
+        => let t := (eval vm_compute in
+                        (Positional.encode (n:=sz) (modulo:=modulo) (div:=div) wt (F.to_Z (m:=M) v))) in
+           (exists t; clear; abstract vm_decide)
+      end.
+
+    Ltac pose_zero_sig m sz wt zero_sig :=
+      assert (zero_sig : { zero : Z^sz | Positional.Fdecode (m:=m) wt zero = 0%F})
+      by solve_constant_sig sz wt.
+
+    Ltac pose_one_sig m sz wt one_sig :=
+      assert (one_sig : { one : Z^sz | Positional.Fdecode (m:=m) wt one = 1%F})
+      by solve_constant_sig sz wt.
+
+    Ltac pose_a24_sig m sz wt a24 a24_sig :=
+      assert (a24_sig : { a24t : Z^sz | Positional.Fdecode (m:=m) wt a24t = F.of_Z m a24 })
+      by solve_constant_sig sz wt.
+
+    Ltac abstract_sig tac :=
+      lazymatch goal with
+      | [ |- sig ?P ]
+        => let H := fresh in
+           transparent assert (H : (sig P)) by (tac ());
+           let Hv := (eval cbv delta [H] in H) in
+           clear -H; clear H;
+           let p1 := (eval cbv [proj1_sig] in (proj1_sig Hv)) in
+           (exists p1);
+           abstract exact (proj2_sig Hv)
+      end.
+
+    Ltac pose_add_sig m sz wt wt_nonzero add_sig :=
+      assert (add_sig
+              : { add : (Z^sz -> Z^sz -> Z^sz)%type |
+                  forall a b : Z^sz,
+                    let eval := Positional.Fdecode (m:=m) wt in
+                    eval (add a b) = (eval a + eval b)%F })
+      by abstract_sig
+           ltac:(fun _ =>
+                   let a := fresh "a" in
+                   let b := fresh "b" in
+                   eexists; cbv beta zeta; intros a b;
+                   generalize wt_nonzero; clear; intro;
+                   let x := constr:(
+                              Positional.add_cps (n := sz) wt a b id) in
+                   solve_op_F wt x;
+                   reflexivity
+                ).
+
+    Ltac pose_sub_sig m sz wt wt_nonzero coef sub_sig :=
+      assert (sub_sig
+              : {sub : (Z^sz -> Z^sz -> Z^sz)%type |
+                 forall a b : Z^sz,
+                   let eval := Positional.Fdecode (m:=m) wt in
+                   eval (sub a b) = (eval a - eval b)%F})
+      by abstract_sig
+           ltac:(fun _ =>
+                   let a := fresh "a" in
+                   let b := fresh "b" in
+                   eexists; cbv beta zeta; intros a b;
+                   generalize wt_nonzero; clear -coef; intro;
+                   let x := constr:(
+                              Positional.sub_cps (n:=sz) (coef := coef) wt a b id) in
+                   solve_op_F wt x;
+                   reflexivity
+                ).
+
+    Ltac pose_opp_sig m sz wt wt_nonzero coef opp_sig :=
+      assert (opp_sig
+              : {opp : (Z^sz -> Z^sz)%type |
+                 forall a : Z^sz,
+                   let eval := Positional.Fdecode (m := m) wt in
+                   eval (opp a) = F.opp (eval a)})
+      by abstract_sig
+           ltac:(fun _ =>
+                   let a := fresh "a" in
+                   eexists; cbv beta zeta; intros a;
+                   generalize wt_nonzero; clear -coef; intro;
+                   let x := constr:(
+                              Positional.opp_cps (n:=sz) (coef := coef) wt a id) in
+                   solve_op_F wt x;
+                   reflexivity
+                ).
+
+    Ltac pose_mul_sig m sz wt wt_nonzero sz2 s c mul_sig :=
+      assert (mul_sig
+              : {mul : (Z^sz -> Z^sz -> Z^sz)%type |
+                 forall a b : Z^sz,
+                   let eval := Positional.Fdecode (m := m) wt in
+                   eval (mul a b) = (eval a * eval b)%F})
+      by abstract_sig
+           ltac:(fun _ =>
+                   let a := fresh "a" in
+                   let b := fresh "b" in
+                   eexists; cbv beta zeta; intros a b;
+                   generalize wt_nonzero; clear -sz2 s c; intro;
+                   let x := constr:(
+                              Positional.mul_cps (n:=sz) (m:=sz2) wt a b
+                                                 (fun ab => Positional.reduce_cps (n:=sz) (m:=sz2) wt s c ab id)) in
+                   solve_op_F wt x;
+                   P.default_mul;
+                   P.extra_prove_mul_eq;
+                   break_match; cbv [Let_In runtime_mul runtime_add]; repeat apply (f_equal2 pair); rewrite ?Z.shiftl_mul_pow2 by omega; ring
+                ).
+
+    Ltac pose_square_sig m sz wt wt_nonzero sz2 s c square_sig :=
+      assert (square_sig
+              : {square : (Z^sz -> Z^sz)%type |
+                 forall a : Z^sz,
+                   let eval := Positional.Fdecode (m := m) wt in
+                   eval (square a) = (eval a * eval a)%F})
+      by abstract_sig
+           ltac:(fun _ =>
+                   let a := fresh "a" in
+                   eexists; cbv beta zeta; intros a;
+                   generalize wt_nonzero; clear -sz2 s c; intro;
+                   let x := constr:(
+                              Positional.mul_cps (n:=sz) (m:=sz2) wt a a
+                                                 (fun ab => Positional.reduce_cps (n:=sz) (m:=sz2) wt s c ab id)) in
+                   solve_op_F wt x;
+                   P.default_square;
+                   P.extra_prove_square_eq;
+                   break_match; cbv [Let_In runtime_mul runtime_add]; repeat apply (f_equal2 pair); rewrite ?Z.shiftl_mul_pow2 by omega; ring
+                ).
+
+    (* Performs a full carry loop (as specified by carry_chain) *)
+    Ltac pose_carry_sig m sz wt wt_nonzero wt_divides_chain1 wt_divides_chain2 carry_chain1 carry_chain2 s c carry_sig :=
+      assert (carry_sig
+              : {carry : (Z^sz -> Z^sz)%type |
+                 forall a : Z^sz,
+                   let eval := Positional.Fdecode (m := m) wt in
+                   eval (carry a) = eval a})
+      by abstract_sig
+           ltac:(fun _ =>
+                   let a := fresh "a" in
+                   eexists; cbv beta zeta; intros a;
+                   generalize wt_divides_chain2; generalize div_mod;
+                   generalize wt_divides_chain1; generalize wt_nonzero;
+                   clear -carry_chain1 carry_chain2 s c; (intros ????);
+                   let x := constr:(
+                              Positional.chained_carries_cps (n:=sz) (div:=div)(modulo:=modulo) wt a carry_chain1
+                                                             (fun r => Positional.carry_reduce_cps (n:=sz) (div:=div) (modulo:=modulo) wt s c r
+                                                                                                   (fun rrr => Positional.chained_carries_cps (n:=sz) (div:=div) (modulo:=modulo) wt rrr carry_chain2 id
+                            ))) in
+                   solve_op_F wt x;
+                   reflexivity
+                ).
+
+    Ltac pose_wt_pos wt wt_pos :=
+      assert (wt_pos : forall i, wt i > 0)
+      by (clear; abstract (eapply pow_ceil_mul_nat_pos; vm_decide)).
+
+    Ltac pose_wt_multiples wt wt_multiples :=
+      assert (wt_multiples : forall i, wt (S i) mod (wt i) = 0)
+      by (clear; abstract (apply pow_ceil_mul_nat_multiples; vm_decide)).
+
+    Ltac pose_freeze_sig m sz wt wt_nonzero wt_pos wt_divides wt_multiples bitwidth m_enc c' freeze_sig :=
+      assert (freeze_sig
+              : {freeze : (Z^sz -> Z^sz)%type |
+                 forall a : Z^sz,
+                   (0 <= Positional.eval wt a < 2 * Z.pos m)->
+                   let eval := Positional.Fdecode (m := m) wt in
+                   eval (freeze a) = eval a})
+      by abstract_sig
+           ltac:(fun _ =>
+                   let a := fresh "a" in
+                   let H := fresh "H" in
+                   eexists; cbv beta zeta; (intros a H);
+                   generalize modulo_correct; generalize div_correct;
+                   generalize wt_multiples;
+                   generalize wt_divides; generalize div_mod;
+                   generalize wt_pos; generalize wt_nonzero;
+                   clear -bitwidth m_enc c' H; (intros ???????);
+                   let x := constr:(freeze (n:=sz) wt (Z.ones bitwidth) m_enc a) in
+                   F_mod_eq;
+                   transitivity (Positional.eval wt x); repeat autounfold;
+                   [ | autorewrite with uncps push_id push_basesystem_eval;
+                       rewrite eval_freeze with (c:=c');
+                       try eassumption; try omega; try reflexivity;
+                       try solve [auto using B.Positional.select_id,
+                                  B.Positional.eval_select, Zselect.Z.zselect_correct];
+                       vm_decide];
+                   cbv[mod_eq]; apply f_equal2;
+                   [  | reflexivity ]; apply f_equal;
+                   cbv - [runtime_opp runtime_add runtime_mul runtime_shr runtime_and Let_In Z.add_get_carry Z.zselect];
+                   reflexivity
+                ).
+
+    Ltac pose_ring m sz wt zero_sig one_sig opp_sig add_sig sub_sig mul_sig sz_nonzero' wt wt_nonzero wt_divides' ring :=
+      pose (Ring.ring_by_isomorphism
+              (F := F m)
+              (H := Z^sz)
+              (phi := Positional.Fencode wt)
+              (phi' := Positional.Fdecode wt)
+              (zero := proj1_sig zero_sig)
+              (one := proj1_sig one_sig)
+              (opp := proj1_sig opp_sig)
+              (add := proj1_sig add_sig)
+              (sub := proj1_sig sub_sig)
+              (mul := proj1_sig mul_sig)
+              (phi'_zero := proj2_sig zero_sig)
+              (phi'_one := proj2_sig one_sig)
+              (phi'_opp := proj2_sig opp_sig)
+              (Positional.Fdecode_Fencode_id
+                 (sz_nonzero := sz_nonzero')
+                 (div_mod := div_mod)
+                 wt eq_refl wt_nonzero wt_divides')
+              (Positional.eq_Feq_iff wt)
+              (proj2_sig add_sig)
+              (proj2_sig sub_sig)
+              (proj2_sig mul_sig)
+           )
+      as ring.
+
+    Local Notation b_of exp := {| lower := 0 ; upper := P.upper_bound_of_exponent exp |}%Z (only parsing). (* max is [(0, 2^(exp+2) + 2^exp + 2^(exp-1) + 2^(exp-3) + 2^(exp-4) + 2^(exp-5) + 2^(exp-6) + 2^(exp-10) + 2^(exp-12) + 2^(exp-13) + 2^(exp-14) + 2^(exp-15) + 2^(exp-17) + 2^(exp-23) + 2^(exp-24))%Z] *)
+    (* The definition [bounds_exp] is a tuple-version of the
+     limb-widths, which are the [exp] argument in [b_of] above, i.e.,
+     the approximate base-2 exponent of the bounds on the limb in that
+     position. *)
+
+    Ltac pose_limb_widths wt sz limb_widths :=
+      let limb_widths' := (eval vm_compute in (List.map (fun i => Z.log2 (wt (S i) / wt i)) (seq 0 sz))) in
+      pose limb_widths' as limb_widths.
+
+    Ltac pose_bounds_exp sz limb_widths bounds_exp :=
+      let bounds_exp' := (eval compute in
+                             (Tuple.from_list sz limb_widths eq_refl)) in
+      pose (bounds_exp' : Tuple.tuple Z sz) as bounds_exp.
+
+    Ltac pose_bounds sz bounds_exp bounds :=
+      let bounds' := (eval compute in
+                         (Tuple.map (fun e => b_of e) bounds_exp)) in
+      pose (bounds' : Tuple.tuple zrange sz) as bounds.
+
+    Ltac pose_lgbitwidth limb_widths lgbitwidth :=
+      let lgbitwidth' := (eval compute in (Z.to_nat (Z.log2_up (List.fold_right Z.max 0 limb_widths)))) in
+      pose lgbitwidth' as lgbitwidth.
+    Ltac pose_adjusted_bitwidth lgbitwidth adjusted_bitwidth :=
+      let adjusted_bitwidth' := (eval compute in (2^lgbitwidth)%nat) in
+      pose adjusted_bitwidth' as adjusted_bitwidth.
+
+    Ltac pose_feZ sz feZ :=
+      pose (tuple Z sz) as feZ.
+    Ltac pose_feW sz lgbitwidth feW :=
+      let feW' := (eval cbv [lgbitwidth] in (tuple (wordT lgbitwidth) sz)) in
+      pose feW' as feW.
+    Ltac pose_feW_bounded bounds feW feW_bounded :=
+      let feW_bounded' := (eval cbv [bounds] in (fun w : feW => is_bounded_by None bounds (Tuple.map wordToZ w))) in
+      pose feW_bounded' as feW_bounded.
+    Ltac pose_feBW adjusted_bitwidth bounds sz feBW :=
+      let feBW' := (eval cbv [adjusted_bitwidth bounds] in (BoundedWord sz adjusted_bitwidth bounds)) in
+      pose feBW' as feBW.
+
+    Ltac pose_phiBW m wt feBW phiBW :=
+      pose (fun x : feBW => (B.Positional.Fdecode wt (BoundedWordToZ _ _ _ x) : F m))
+      as phiBW.
+
+    Ltac pose_phiW m wt feW phiW :=
+      pose (fun x : feW => (B.Positional.Fdecode wt (Tuple.map wordToZ x) : F m))
+      as phiW.
+
+    Ltac pose_feBW_bounded m sz wt adjusted_bitwidth bounds feBW feBW_bounded :=
+      assert (feBW_bounded : forall (a : feBW),
+                 0 <= B.Positional.eval wt (BoundedWordToZ sz adjusted_bitwidth bounds a) < 2 * Z.pos m)
+      by (clear;
+          abstract (
+              let a := fresh "a" in
+              let H := fresh "H" in
+              intros a;
+              destruct a as [a H]; unfold BoundedWordToZ, proj1_sig;
+              revert H;
+              cbv -[Z.le Z.add Z.mul Z.lt fst snd wordToZ wt]; cbn [fst snd];
+              repeat match goal with
+                     | [ |- context[wt ?n] ]
+                       => let v := (eval compute in (wt n)) in change (wt n) with v
+                     end;
+              intro; destruct_head'_and;
+              omega
+            )).
+
+    Ltac pose_allowable_bit_widths allowable_bit_widths :=
+      pose_computed P.allowable_bit_widths allowable_bit_widths.
+    Ltac pose_freeze_allowable_bit_widths freeze_allowable_bit_widths :=
+      pose_computed P.freeze_allowable_bit_widths freeze_allowable_bit_widths.
+  End Internal.
+
+  Ltac synthesize _ :=
+    let sz := fresh "sz" in
+    let bitwidth := fresh "bitwidth" in
+    let s := fresh "s" in
+    let c := fresh "c" in
+    let carry_chain1 := fresh "carry_chain1" in
+    let carry_chain2 := fresh "carry_chain2" in
+    let a24 := fresh "a24" in
+    let coef_div_modulus := fresh "coef_div_modulus" in
+    let m := fresh "m" in
+    let wt := fresh "wt" in
+    let sz2 := fresh "sz2" in
+    let m_enc := fresh "m_enc" in
+    let coef := fresh "coef" in
+    let coef_mod := fresh "coef_mod" in
+    let sz_nonzero := fresh "sz_nonzero" in
+    let wt_nonzero := fresh "wt_nonzero" in
+    let wt_divides := fresh "wt_divides" in
+    let wt_divides' := fresh "wt_divides'" in
+    let wt_divides_chain1 := fresh "wt_divides_chain1" in
+    let wt_divides_chain2 := fresh "wt_divides_chain2" in
+    let zero_sig := fresh "zero_sig" in
+    let one_sig := fresh "one_sig" in
+    let a24_sig := fresh "a24_sig" in
+    let add_sig := fresh "add_sig" in
+    let sub_sig := fresh "sub_sig" in
+    let opp_sig := fresh "opp_sig" in
+    let mul_sig := fresh "mul_sig" in
+    let square_sig := fresh "square_sig" in
+    let carry_sig := fresh "carry_sig" in
+    let wt_pos := fresh "wt_pos" in
+    let wt_multiples := fresh "wt_multiples" in
+    let freeze_sig := fresh "freeze_sig" in
+    let ring := fresh "ring" in
+    let limb_widths := fresh "limb_widths" in
+    let bounds_exp := fresh "bounds_exp" in
+    let bounds := fresh "bounds" in
+    let lgbitwidth := fresh "lgbitwidth" in
+    let adjusted_bitwidth := fresh "adjusted_bitwidth" in
+    let feZ := fresh "feZ" in
+    let feW := fresh "feW" in
+    let feW_bounded := fresh "feW_bounded" in
+    let feBW := fresh "feBW" in
+    let feBW_bounded := fresh "feBW_bounded" in
+    let phiBW := fresh "phiBW" in
+    let phiW := fresh "phiW" in
+    let allowable_bit_widths := fresh "allowable_bit_widths" in
+    let freeze_allowable_bit_widths := fresh "freeze_allowable_bit_widths" in
+    pose_sz sz;
+    pose_bitwidth bitwidth;
+    pose_s s;
+    pose_c c;
+    pose_carry_chain1 carry_chain1;
+    pose_carry_chain2 carry_chain2;
+    pose_a24 a24;
+    pose_coef_div_modulus coef_div_modulus;
+    pose_m s c m;
+    pose_wt m sz wt;
+    pose_sz2 sz sz2;
+    pose_m_enc sz wt s c m_enc;
+    pose_coef sz wt m_enc coef_div_modulus coef;
+    pose_coef_mod m sz wt coef coef_mod;
+    pose_sz_nonzero sz sz_nonzero;
+    pose_wt_nonzero wt wt_nonzero;
+    pose_wt_divides wt wt_divides;
+    pose_wt_divides' wt wt_divides wt_divides';
+    pose_wt_divides_chain carry_chain1 wt wt_divides' wt_divides_chain1;
+    pose_wt_divides_chain carry_chain2 wt wt_divides' wt_divides_chain2;
+    pose_zero_sig m sz wt zero_sig;
+    pose_one_sig m sz wt one_sig;
+    pose_a24_sig m sz wt a24 a24_sig;
+    pose_add_sig m sz wt wt_nonzero add_sig;
+    pose_sub_sig m sz wt wt_nonzero coef sub_sig;
+    pose_opp_sig m sz wt wt_nonzero coef opp_sig;
+    pose_mul_sig m sz wt wt_nonzero sz2 s c mul_sig;
+    pose_square_sig m sz wt wt_nonzero sz2 s c square_sig;
+    pose_carry_sig m sz wt wt_nonzero wt_divides_chain1 wt_divides_chain2 carry_chain1 carry_chain2 s c carry_sig;
+    pose_wt_pos wt wt_pos;
+    pose_wt_multiples wt wt_multiples;
+    pose_freeze_sig m sz wt wt_nonzero wt_pos wt_divides wt_multiples bitwidth m_enc c freeze_sig;
+    pose_ring m sz wt zero_sig one_sig opp_sig add_sig sub_sig mul_sig sz_nonzero wt wt_nonzero wt_divides' ring;
+    pose_limb_widths wt sz limb_widths;
+    pose_bounds_exp sz limb_widths bounds_exp;
+    pose_bounds sz bounds_exp bounds;
+    pose_lgbitwidth limb_widths lgbitwidth;
+    pose_adjusted_bitwidth lgbitwidth adjusted_bitwidth;
+    pose_feZ sz feZ;
+    pose_feW sz lgbitwidth feW;
+    pose_feW_bounded bounds feW feW_bounded;
+    pose_feBW adjusted_bitwidth bounds sz feBW;
+    pose_feBW_bounded m sz wt adjusted_bitwidth bounds feBW feBW_bounded;
+    pose_phiBW m wt feBW phiBW;
+    pose_phiW m wt feW phiW;
+    pose_allowable_bit_widths allowable_bit_widths;
+    pose_freeze_allowable_bit_widths freeze_allowable_bit_widths;
+    let do_refine_package _ :=
+        simple refine {|
+                 ASPackage :=
+                   (@Build_ArithmeticSynthesisTestPackage'
+                      ({|
+                          m := m;
+                          sz := sz;
+                          a24 := a24;
+                          lgbitwidth := lgbitwidth;
+                          adjusted_bitwidth := adjusted_bitwidth;
+                          bounds := bounds;
+                          allowable_bit_widths := allowable_bit_widths;
+                          freeze_allowable_bit_widths := freeze_allowable_bit_widths;
+                        |})
+                      a24_sig
+                      add_sig
+                      sub_sig
+                      opp_sig
+                      mul_sig
+                      square_sig
+                      carry_sig
+                      freeze_sig
+                      feW_bounded
+                      (BoundedWordToZ sz adjusted_bitwidth bounds)
+                      feBW_bounded)
+               |} in
+    lazymatch goal with
+    | [ |- ArithmeticSynthesisTestPackage ]
+      => do_refine_package ()
+    | [ |- ?e ]
+      => tryif is_evar e then do_refine_package () else idtac
+    | _ => idtac
+    end.
+End Synthesize.
+
+(*
+Eval cbv [proj1_sig add_sig] in (proj1_sig add_sig).
+Eval cbv [proj1_sig sub_sig] in (proj1_sig sub_sig).
+Eval cbv [proj1_sig opp_sig] in (proj1_sig opp_sig).
+Eval cbv [proj1_sig mul_sig] in (proj1_sig mul_sig).
+Eval cbv [proj1_sig carry_sig] in (proj1_sig carry_sig).
+*)
+
+(* Require Import Crypto.Specific.X25519.C64.CurveParameters.
+
+Module S := Synthesize Curve.
+
+Definition synthesized' : ArithmeticSynthesisTestPackage.
+Proof. Time S.synthesize (). Time Defined.
+
+Time Definition synthesized :=
+  Eval cbv zeta delta [synthesized'] in synthesized'.
+*)
