src/Specific/ArithmeticSynthesisReflectiveFrameworkLadderstep.v
@@ -1,0 +1,163 @@
+Require Import Coq.Classes.Morphisms.
+
+Require Import Crypto.Arithmetic.Core.
+Require Import Crypto.Arithmetic.PrimeFieldTheorems.
+Require Import Crypto.Util.BoundedWord.
+Require Import Crypto.Specific.IntegrationTestTemporaryMiscCommon.
+Require Import Crypto.Compilers.Z.Bounds.Pipeline.
+Require Import Crypto.Specific.ArithmeticSynthesisFramework.
+
+Require Import Crypto.Util.FixedWordSizes.
+Require Import Coq.ZArith.BinIntDef.
+Require Import Crypto.Curves.Montgomery.XZ.
+Require Import Crypto.Util.Sigma.MapProjections Crypto.Util.Sigma.Lift.
+Require Import Crypto.Util.Tuple.
+Require Import Crypto.Util.LetIn.
+Require Import Crypto.Util.Tactics.Head.
+Require Import Crypto.Util.Tactics.MoveLetIn.
+Require Import Crypto.Util.Tactics.SetEvars.
+Require Import Crypto.Util.Tactics.SubstEvars.
+Require Import Crypto.Util.Tactics.ETransitivity.
+Require Import Crypto.Util.Notations.
+
+Section with_package.
+  Context (package : ArithmeticSynthesisTestPackage).
+
+  Local Notation add_sig := (@add_sig _ package).
+  Local Notation mul_sig := (@mul_sig _ package).
+  Local Notation carry_sig := (@carry_sig _ package).
+  Local Notation sub_sig := (@sub_sig _ package).
+  Local Notation square_sig := (@square_sig _ package).
+  Local Notation tuple := Tuple.tuple.
+
+  (** TODO(jadep,andreser): Move to NewBaseSystemTest? *)
+  Definition FMxzladderstep := @M.donnaladderstep (F m) F.add F.sub F.mul.
+
+  Section with_notations.
+    Local Infix "+" := (proj1_sig add_sig).
+    Local Notation "a * b" := (proj1_sig carry_sig (proj1_sig mul_sig a b)).
+    Local Notation "x ^ 2" := (proj1_sig carry_sig (proj1_sig square_sig x)).
+    Local Infix "-" := (proj1_sig sub_sig).
+    Definition Mxzladderstep a24 x1 Q Q'
+      := match Q, Q' with
+         | (x, z), (x', z') =>
+           dlet origx := x in
+           dlet x := x + z in
+           dlet z := origx - z in
+           dlet origx' := x' in
+           dlet x' := x' + z' in
+           dlet z' := origx' - z' in
+           dlet xx' := x' * z in
+           dlet zz' := x * z' in
+           dlet origx' := xx' in
+           dlet xx' := xx' + zz' in
+           dlet zz' := origx' - zz' in
+           dlet x3 := xx'^2 in
+           dlet zzz' := zz'^2 in
+           dlet z3 := zzz' * x1 in
+           dlet xx := x^2 in
+           dlet zz := z^2 in
+           dlet x2 := xx * zz in
+           dlet zz := xx - zz in
+           dlet zzz := zz * a24 in
+           dlet zzz := zzz + xx in
+           dlet z2 := zz * zzz in
+           ((x2, z2), (x3, z3))%core
+         end.
+  End with_notations.
+
+  (** TODO(jadep,andreser): Move to NewBaseSystemTest? *)
+  Definition Mxzladderstep_sig
+    : { xzladderstep : tuple Z sz -> tuple Z sz -> tuple Z sz * tuple Z sz -> tuple Z sz * tuple Z sz -> tuple Z sz * tuple Z sz * (tuple Z sz * tuple Z sz)
+      | forall a24 x1 Q Q', let eval := B.Positional.Fdecode wt in Tuple.map (n:=2) (Tuple.map (n:=2) eval) (xzladderstep a24 x1 Q Q') = FMxzladderstep (eval a24) (eval x1) (Tuple.map (n:=2) eval Q) (Tuple.map (n:=2) eval Q') }.
+  Proof.
+    exists Mxzladderstep.
+    intros a24 x1 Q Q' eval.
+    cbv [Mxzladderstep FMxzladderstep M.donnaladderstep].
+    destruct Q, Q'; cbv [Tuple.map Tuple.map' fst snd Let_In eval].
+    repeat rewrite ?(proj2_sig add_sig), ?(proj2_sig mul_sig), ?(proj2_sig square_sig), ?(proj2_sig sub_sig), ?(proj2_sig carry_sig).
+    reflexivity.
+  Defined.
+End with_package.
+
+Ltac assert_xzladderstep_then package xzladderstep cont :=
+  let feW' := fresh "feW'" in
+  let feW_bounded' := fresh "feW_bounded'" in
+  let phi' := fresh "phi'" in
+  let a24_sig' := fresh "a24_sig'" in
+  let FMxzladderstep' := fresh "FMxzladderstep'" in
+  let wt' := fresh "wt'" in
+  pose (@feW _ package) as feW';
+  pose (@feW_bounded _ package) as feW_bounded';
+  pose (@phiW _ package) as phi';
+  pose (@a24_sig _ package) as a24_sig';
+  pose (@FMxzladderstep package) as FMxzladderstep';
+  pose (@wt _ package) as wt';
+  assert (xzladderstep
+          : { xzladderstep : feW' -> feW' * feW' -> feW' * feW' -> feW' * feW' * (feW' * feW')
+            | forall x1 Q Q',
+                let xz := xzladderstep x1 Q Q' in
+                let eval := B.Positional.Fdecode wt' in
+                feW_bounded' x1
+                -> feW_bounded' (fst Q) /\ feW_bounded' (snd Q)
+                -> feW_bounded' (fst Q') /\ feW_bounded' (snd Q')
+                -> ((feW_bounded' (fst (fst xz)) /\ feW_bounded' (snd (fst xz)))
+                    /\ (feW_bounded' (fst (snd xz)) /\ feW_bounded' (snd (snd xz))))
+                   /\ Tuple.map (n:=2) (Tuple.map (n:=2) phi') xz = FMxzladderstep' (eval (proj1_sig a24_sig')) (phi' x1) (Tuple.map (n:=2) phi' Q) (Tuple.map (n:=2) phi' Q') });
+  [ cont feW' feW_bounded' phi' a24_sig' FMxzladderstep' wt'
+  | cbv delta [feW' feW_bounded' phi' a24_sig' FMxzladderstep' wt'] in xzladderstep;
+    clear feW' feW_bounded' phi' a24_sig' FMxzladderstep' wt' ].
+
+Ltac preglue_xzladderstep package feW' feW_bounded' phi' a24_sig' FMxzladderstep' wt' :=
+  let Mxzladderstep_sig' := fresh "Mxzladderstep_sig'" in
+  pose (@Mxzladderstep_sig package) as Mxzladderstep_sig';
+  let a := fresh "a" in
+  let b := fresh "b" in
+  let c := fresh "c" in
+  cbv [phiW] in phi';
+  apply_lift_sig;
+  intros a b c; cbv beta iota zeta;
+  lazymatch goal with
+  | [ |- { e | ?A -> ?B -> ?C -> @?E e } ]
+    => refine (proj2_sig_map (P:=fun e => A -> B -> C -> (_:Prop)) _ _)
+  end;
+  [ let FINAL := fresh "FINAL" in
+    intros ? FINAL;
+    repeat (let H := fresh in intro H; specialize (FINAL H));
+    cbv [phi'];
+    split; [ refine (proj1 FINAL); shelve | ];
+    do 4 match goal with
+         | [ |- context[Tuple.map (n:=?N) (fun x : ?T => ?f (?g x))] ]
+           => rewrite <- (Tuple.map_map (n:=N) f g
+                          : pointwise_relation _ eq _ (Tuple.map (n:=N) (fun x : T => f (g x))))
+         end;
+    rewrite <- (proj2_sig Mxzladderstep_sig');
+    apply f_equal;
+    cbv [proj1_sig]; cbv [Mxzladderstep_sig' Mxzladderstep_sig];
+    context_to_dlet_in_rhs (@Mxzladderstep _ _);
+    hnf in a24_sig';
+    cbv [Mxzladderstep a24_sig'];
+    repeat lazymatch goal with
+           | [ |- context[@proj1_sig ?a ?b ?f_sig _] ]
+             => context_to_dlet_in_rhs (@proj1_sig a b f_sig)
+           end;
+    cbv [sz ASParams ASPackage lgbitwidth package wt_gen
+            proj1_sig mul_sig add_sig sub_sig carry_sig square_sig];
+    cbv_runtime;
+    refine (proj2 FINAL)
+  | ];
+  clear phi' a24_sig' FMxzladderstep' Mxzladderstep_sig' wt';
+  cbv [feW' feW_bounded' feW feW_bounded
+            ASParams ASPackage package lgbitwidth sz] in *;
+  clear feW' feW_bounded'.
+
+Ltac refine_reflectively_xzladderstep package :=
+  let allowable_bit_widths := constr:(@allowable_bit_widths package) in
+  refine_reflectively_gen allowable_bit_widths default.
+
+Ltac pose_xzladderstep package xzladderstep :=
+  assert_xzladderstep_then
+    package xzladderstep
+    ltac:(fun feW' feW_bounded' phi' a24_sig' FMxzladderstep' wt'
+          => preglue_xzladderstep package feW' feW_bounded' phi' a24_sig' FMxzladderstep' wt';
+             refine_reflectively_xzladderstep package).
